Finish rebase, everything working

Staged.v
@@ -4,17 +4,13 @@ From Coq Require Import Classes.RelationClasses.
 
 Set Implicit Arguments.
 From SLF Require Export LibString LibCore.
-(* From SLF Require Export LibSepFmap. *)
 From SLF Require Export LibSepTLCbuffer LibSepFmap.
 Module Fmap := LibSepFmap.
-(* From SLF Require Heap. *)
-(* From SLF Require Export Heap. *)
-(* From SLF Require Export LibSepMinimal. *)
+From SLF Require LibSepSimpl.
 
 From SLF Require Import Tactics.
 
 (* From CDF Require Import Common Sequences Separation Tactics HeapTactics. *)
-
 
 Local Open Scope string_scope.
 (* Local Open Scope nat_scope. *)
@@ -73,6 +69,7 @@ Inductive eresult : Type :=
 Definition loc : Type := nat.
 Definition heap : Type := fmap loc val.
 
+Definition empty_heap : heap := Fmap.empty.
 
 
 (* Reserved Notation " 'eval[' s ',' h ',' e ']' '=>' '[' s1 ',' h1 ',' r ']' " (at level 50, left associativity). *)
@@ -136,71 +133,66 @@ Module ProgramExamples.
 
 End ProgramExamples.
 
-(* copied from LibSepMinimal *)
+(* copied from LibSepReference *)
 
-Implicit Types Q : val->heap->Prop.
-
-(* ================================================================= *)
-(** ** Automation for Heap Equality and Heap Disjointness *)
-
-(** For goals asserting equalities between heaps, i.e., of the form [h1 = h2],
-    we set up automation so that it performs some tidying: substitution,
-    removal of empty heaps, normalization with respect to associativity. *)
-
-#[global] Hint Rewrite union_assoc union_empty_l union_empty_r : fmap.
-#[global] Hint Extern 1 (_ = _ :> heap) => subst; autorewrite with fmap.
-
-(** For goals asserting disjointness between heaps, i.e., of the form
-    [Fmap.disjoint h1 h2], we set up automation to perform simplifications:
-    substitution, exploit distributivity of the disjointness predicate over
-    unions of heaps, and exploit disjointness with empty heaps. The tactic
-    [jauto_set] used here comes from the TLC library; essentially, it destructs
-    conjunctions and existentials. *)
-
-#[global] Hint Resolve Fmap.disjoint_empty_l Fmap.disjoint_empty_r.
-#[global] Hint Rewrite disjoint_union_eq_l disjoint_union_eq_r : disjoint.
-#[global] Hint Extern 1 (Fmap.disjoint _ _) =>
-  subst; autorewrite with rew_disjoint in *; jauto_set.
+Notation "h1 \u h2" := (Fmap.union h1 h2)
+  (at level 37, right associativity).
 
 (* ################################################################# *)
-(** * Heap Predicates and Entailment *)
+(** * Heap Predicates *)
+
+(** We next define heap predicates and establish their properties. All this
+    material is wrapped in a module, allowing us to instantiate the functor from
+    chapter [LibSepSimpl] that defines the tactic [xsimpl]. *)
+Module SepSimplArgs.
 
 (* ================================================================= *)
-(** ** Extensionality Axioms *)
+(** ** Hprop and Entailment *)
 
-(** Extensionality axioms are essential to assert equalities between heap
-    predicates of type [hprop], and between postconditions, of type
-    [val->hprop]. *)
-
-Axiom functional_extensionality : forall A B (f g:A->B),
-  (forall x, f x = g x) ->
-  f = g.
-
-Axiom propositional_extensionality : forall (P Q:Prop),
-  (P <-> Q) ->
-  P = Q.
-
-(* ================================================================= *)
-(** ** Core Heap Predicates *)
+Declare Scope hprop_scope.
+Open Scope hprop_scope.
 
 (** The type of heap predicates is named [hprop]. *)
 
 Definition hprop := heap -> Prop.
 
-(** We bind a few more meta-variables. *)
+(** Implicit types for meta-variables. *)
 
 Implicit Types P : Prop.
 Implicit Types H : hprop.
+Implicit Types Q : val->hprop.
 
-(** Core heap predicates, and their associated notations:
+(** Entailment for heap predicates, written [H1 ==> H2]. This entailment
+    is linear. *)
+
+Definition himpl (H1 H2:hprop) : Prop :=
+  forall h, H1 h -> H2 h.
+
+Notation "H1 ==> H2" := (himpl H1 H2) (at level 55) : hprop_scope.
+
+(** Entailment between postconditions, written [Q1 ===> Q2]. *)
+
+Definition qimpl A (Q1 Q2:A->hprop) : Prop :=
+  forall (v:A), Q1 v ==> Q2 v.
+
+Notation "Q1 ===> Q2" := (qimpl Q1 Q2) (at level 55) : hprop_scope.
+
+(* ================================================================= *)
+(** ** Definition of Heap Predicates *)
+
+(** The core heap predicates are defined next, together with the
+    associated notation:
 
     - [\[]] denotes the empty heap predicate
     - [\[P]] denotes a pure fact
+    - [\Top] denotes the true heap predicate (affine)
     - [p ~~> v] denotes a singleton heap
     - [H1 \* H2] denotes the separating conjunction
     - [Q1 \*+ H2] denotes the separating conjunction extending a postcondition
-    - [\exists x, H] denotes an existential
-    - [\forall x, H] denotes a universal. *)
+    - [\exists x, H] denotes an existential quantifier
+    - [\forall x, H] denotes a universal quantifier
+    - [H1 \-* H2] denotes a magic wand between heap predicates
+    - [Q1 \--* Q2] denotes a magic wand between postconditions. *)
 
 Definition hempty : hprop :=
   fun h => (h = Fmap.empty).
@@ -220,24 +212,13 @@ Definition hexists A (J:A->hprop) : hprop :=
 Definition hforall (A : Type) (J : A -> hprop) : hprop :=
   fun h => forall x, J x h.
 
-Definition hpure (P:Prop) : hprop := (* encoded as [\exists (p:P), \[]] *)
-  hexists (fun (p:P) => hempty).
-
-Declare Scope hprop_scope.
-
 Notation "\[]" := (hempty)
   (at level 0) : hprop_scope.
-
-Notation "\[ P ]" := (hpure P)
-  (at level 0, format "\[ P ]") : hprop_scope.
 
 Notation "p '~~>' v" := (hsingle p v) (at level 32) : hprop_scope.
 
 Notation "H1 '\*' H2" := (hstar H1 H2)
   (at level 41, right associativity) : hprop_scope.
-
-Notation "Q \*+ H" := (fun x => hstar (Q x) H)
-  (at level 40) : hprop_scope.
 
 Notation "'\exists' x1 .. xn , H" :=
   (hexists (fun x1 => .. (hexists (fun xn => H)) ..))
@@ -249,231 +230,603 @@ Notation "'\forall' x1 .. xn , H" :=
   (at level 39, x1 binder, H at level 50, right associativity,
    format "'[' '\forall' '/ '  x1  ..  xn , '/ '  H ']'") : hprop_scope.
 
+(** The remaining operators are defined in terms of the preivous above,
+    rather than directly as functions over heaps. Doing so reduces the
+    amount of proofs, by allowing to better leverage the tactic [xsimpl]. *)
+
+Definition hpure (P:Prop) : hprop :=
+  \exists (p:P), \[].
+
+Definition htop : hprop :=
+  \exists (H:hprop), H.
+
+Definition hwand (H1 H2 : hprop) : hprop :=
+  \exists H0, H0 \* hpure ((H1 \* H0) ==> H2).
+
+Definition qwand A (Q1 Q2:A->hprop) : hprop :=
+  \forall x, hwand (Q1 x) (Q2 x).
+
+Notation "\[ P ]" := (hpure P)
+  (at level 0, format "\[ P ]") : hprop_scope.
+
+Notation "\Top" := (htop) : hprop_scope.
+
+Notation "Q \*+ H" := (fun x => hstar (Q x) H)
+  (at level 40) : hprop_scope.
+
+Notation "H1 \-* H2" := (hwand H1 H2)
+  (at level 43, right associativity) : hprop_scope.
+
+Notation "Q1 \--* Q2" := (qwand Q1 Q2)
+  (at level 43) : hprop_scope.
+
 (* ================================================================= *)
-(** ** Entailment *)
+(** ** Basic Properties of Separation Logic Operators *)
 
-Declare Scope hprop_scope.
-Open Scope hprop_scope.
+(* ----------------------------------------------------------------- *)
+(** *** Tactic for Automation *)
 
-(** Entailment for heap predicates, written [H1 ==> H2]. *)
+(** We set up [auto] to process goals of the form [h1 = h2] by calling
+    [fmap_eq], which proves equality modulo associativity and commutativity. *)
 
-Definition himpl (H1 H2:hprop) : Prop :=
-  forall h, H1 h -> H2 h.
+#[global] Hint Extern 1 (_ = _ :> heap) => fmap_eq.
 
-Notation "H1 ==> H2" := (himpl H1 H2) (at level 55) : hprop_scope.
+(** We also set up [auto] to process goals of the form [Fmap.disjoint h1 h2]
+    by calling the tactic [fmap_disjoint], which essentially normalizes all
+    disjointness goals and hypotheses, split all conjunctions, and invokes
+    proof search with a base of hints specified in [LibSepFmap.v]. *)
 
-(** Entailment between postconditions, written [Q1 ===> Q2] *)
+Import Fmap.DisjointHints.
 
-Definition qimpl A (Q1 Q2:A->hprop) : Prop :=
-  forall (v:A), Q1 v ==> Q2 v.
+Tactic Notation "fmap_disjoint_pre" :=
+  subst; rew_disjoint; jauto_set.
 
-Notation "Q1 ===> Q2" := (qimpl Q1 Q2) (at level 55) : hprop_scope.
+#[global] Hint Extern 1 (Fmap.disjoint _ _) => fmap_disjoint_pre.
 
-(** Entailment defines an order on heap predicates *)
+(* ----------------------------------------------------------------- *)
+(** *** Properties of [himpl] and [qimpl] *)
 
 Lemma himpl_refl : forall H,
   H ==> H.
-Proof. introv M. auto. Qed.
+Proof using. introv M. auto. Qed.
+
+#[global] Hint Resolve himpl_refl.
 
 Lemma himpl_trans : forall H2 H1 H3,
   (H1 ==> H2) ->
   (H2 ==> H3) ->
   (H1 ==> H3).
-Proof. introv M1 M2. unfolds* himpl. Qed.
+Proof using. introv M1 M2. unfolds* himpl. Qed.
+
+Lemma himpl_trans_r : forall H2 H1 H3,
+   H2 ==> H3 ->
+   H1 ==> H2 ->
+   H1 ==> H3.
+Proof using. introv M1 M2. applys* himpl_trans M2 M1. Qed.
 
 Lemma himpl_antisym : forall H1 H2,
   (H1 ==> H2) ->
   (H2 ==> H1) ->
   (H1 = H2).
-Proof. introv M1 M2. applys pred_ext_1. intros h. iff*. Qed.
+Proof using. introv M1 M2. applys pred_ext_1. intros h. iff*. Qed.
 
-Lemma qimpl_refl : forall Q,
+Lemma hprop_op_comm : forall (op:hprop->hprop->hprop),
+  (forall H1 H2, op H1 H2 ==> op H2 H1) ->
+  (forall H1 H2, op H1 H2 = op H2 H1).
+Proof using. introv M. intros. applys himpl_antisym; applys M. Qed.
+
+Lemma qimpl_refl : forall A (Q:A->hprop),
   Q ===> Q.
-Proof. intros Q v. applys himpl_refl. Qed.
+Proof using. intros. unfolds*. Qed.
 
-#[global] Hint Resolve himpl_refl qimpl_refl.
+#[global] Hint Resolve qimpl_refl.
 
-(* ================================================================= *)
-(** ** Properties of [hstar] *)
+(* ----------------------------------------------------------------- *)
+(** *** Properties of [hempty] *)
+
+Lemma hempty_intro :
+  \[] Fmap.empty.
+Proof using. unfolds*. Qed.
+
+Lemma hempty_inv : forall h,
+  \[] h ->
+  h = Fmap.empty.
+Proof using. auto. Qed.
+
+(* ----------------------------------------------------------------- *)
+(** *** Properties of [hstar] *)
 
 Lemma hstar_intro : forall H1 H2 h1 h2,
   H1 h1 ->
   H2 h2 ->
   Fmap.disjoint h1 h2 ->
   (H1 \* H2) (Fmap.union h1 h2).
-Proof. intros. exists* h1 h2. Qed.
+Proof using. intros. exists~ h1 h2. Qed.
+
+Lemma hstar_inv : forall H1 H2 h,
+  (H1 \* H2) h ->
+  exists h1 h2, H1 h1 /\ H2 h2 /\ Fmap.disjoint h1 h2 /\ h = Fmap.union h1 h2.
+Proof using. introv M. applys M. Qed.
 
 Lemma hstar_comm : forall H1 H2,
    H1 \* H2 = H2 \* H1.
-Proof.
-  unfold hprop, hstar. intros H1 H2. applys himpl_antisym.
-  { intros h (h1&h2&M1&M2&D&U).
-    rewrite* Fmap.union_comm_of_disjoint in U. exists* h2 h1. }
-  { intros h (h1&h2&M1&M2&D&U).
-    rewrite* Fmap.union_comm_of_disjoint in U. exists* h2 h1. }
+Proof using.
+  applys hprop_op_comm. unfold hprop, hstar. intros H1 H2.
+  intros h (h1&h2&M1&M2&D&U). rewrite~ Fmap.union_comm_of_disjoint in U.
+  exists* h2 h1.
 Qed.
 
 Lemma hstar_assoc : forall H1 H2 H3,
   (H1 \* H2) \* H3 = H1 \* (H2 \* H3).
-Proof.
+Proof using.
   intros H1 H2 H3. applys himpl_antisym; intros h.
   { intros (h'&h3&(h1&h2&M3&M4&D'&U')&M2&D&U). subst h'.
-    exists h1 (h2 \+ h3). splits*. { applys* hstar_intro. } }
+    exists h1 (h2 \+ h3). splits~. { applys* hstar_intro. } }
   { intros (h1&h'&M1&(h2&h3&M3&M4&D'&U')&D&U). subst h'.
-    exists (h1 \+ h2) h3. splits*. { applys* hstar_intro. } }
+    exists (h1 \+ h2) h3. splits~. { applys* hstar_intro. } }
 Qed.
 
 Lemma hstar_hempty_l : forall H,
   \[] \* H = H.
-Proof.
+Proof using.
   intros. applys himpl_antisym; intros h.
-  { intros (h1&h2&M1&M2&D&U). hnf in M1. subst. rewrite* Fmap.union_empty_l. }
-  { intros M. exists (@Fmap.empty loc val) h. splits*. { hnfs*. } }
+  { intros (h1&h2&M1&M2&D&U). forwards E: hempty_inv M1. subst.
+    rewrite~ Fmap.union_empty_l. }
+  { intros M. exists (Fmap.empty:heap) h. splits~. { applys hempty_intro. } }
+Qed.
+
+Lemma hstar_hempty_r : forall H,
+  H \* \[] = H.
+Proof using.
+  applys neutral_r_of_comm_neutral_l. applys~ hstar_comm. applys~ hstar_hempty_l.
 Qed.
 
 Lemma hstar_hexists : forall A (J:A->hprop) H,
   (hexists J) \* H = hexists (fun x => (J x) \* H).
-Proof.
+Proof using.
   intros. applys himpl_antisym; intros h.
-  { intros (h1&h2&(x&M1)&M2&D&U). exists* x h1 h2. }
-  { intros (x&(h1&h2&M1&M2&D&U)). exists h1 h2. splits*. { exists* x. } }
+  { intros (h1&h2&(x&M1)&M2&D&U). exists~ x h1 h2. }
+  { intros (x&(h1&h2&M1&M2&D&U)). exists h1 h2. splits~. { exists~ x. } }
 Qed.
 
 Lemma hstar_hforall : forall H A (J:A->hprop),
   (hforall J) \* H ==> hforall (J \*+ H).
-Proof.
-  intros. intros h M. destruct M as (h1&h2&M1&M2&D&U). intros x. exists* h1 h2.
+Proof using.
+  intros. intros h M. destruct M as (h1&h2&M1&M2&D&U). intros x. exists~ h1 h2.
 Qed.
 
 Lemma himpl_frame_l : forall H2 H1 H1',
   H1 ==> H1' ->
   (H1 \* H2) ==> (H1' \* H2).
-Proof. introv W (h1&h2&?). exists* h1 h2. Qed.
-
-(** Additional, symmetric results, useful for tactics *)
-
-Lemma hstar_hempty_r : forall H,
-  H \* \[] = H.
-Proof.
-  applys neutral_r_of_comm_neutral_l. applys* hstar_comm. applys* hstar_hempty_l.
-Qed.
+Proof using. introv W (h1&h2&?). exists* h1 h2. Qed.
 
 Lemma himpl_frame_r : forall H1 H2 H2',
   H2 ==> H2' ->
   (H1 \* H2) ==> (H1 \* H2').
-Proof.
-  introv M. do 2 rewrite (@hstar_comm H1). applys* himpl_frame_l.
+Proof using.
+  introv M. do 2 rewrite (@hstar_comm H1). applys~ himpl_frame_l.
 Qed.
 
-(* ================================================================= *)
-(** ** Properties of [hpure] *)
+Lemma himpl_frame_lr : forall H1 H1' H2 H2',
+  H1 ==> H1' ->
+  H2 ==> H2' ->
+  (H1 \* H2) ==> (H1' \* H2').
+Proof using.
+  introv M1 M2. applys himpl_trans. applys~ himpl_frame_l M1. applys~ himpl_frame_r.
+Qed.
+
+Lemma himpl_hstar_trans_l : forall H1 H2 H3 H4,
+  H1 ==> H2 ->
+  H2 \* H3 ==> H4 ->
+  H1 \* H3 ==> H4.
+Proof using.
+  introv M1 M2. applys himpl_trans M2. applys himpl_frame_l M1.
+Qed.
+
+Lemma himpl_hstar_trans_r : forall H1 H2 H3 H4,
+  H1 ==> H2 ->
+  H3 \* H2 ==> H4 ->
+  H3 \* H1 ==> H4.
+Proof using.
+  introv M1 M2. applys himpl_trans M2. applys himpl_frame_r M1.
+Qed.
+
+(* ----------------------------------------------------------------- *)
+(** ***  Properties of [hpure] *)
+
+Lemma hpure_intro : forall P,
+  P ->
+  \[P] Fmap.empty.
+Proof using. introv M. exists M. unfolds*. Qed.
+
+Lemma hpure_inv : forall P h,
+  \[P] h ->
+  P /\ h = Fmap.empty.
+Proof using. introv (p&M). split~. Qed.
 
 Lemma hstar_hpure_l : forall P H h,
   (\[P] \* H) h = (P /\ H h).
-Proof.
+Proof using.
   intros. apply prop_ext. unfold hpure.
   rewrite hstar_hexists. rewrite* hstar_hempty_l.
-  iff (p&M) (p&M). { split*. } { exists* p. }
+  iff (p&M) (p&M). { split~. } { exists~ p. }
+Qed.
+
+Lemma hstar_hpure_r : forall P H h,
+  (H \* \[P]) h = (H h /\ P).
+Proof using.
+  intros. rewrite hstar_comm. rewrite hstar_hpure_l. apply* prop_ext.
 Qed.
 
 Lemma himpl_hstar_hpure_r : forall P H H',
   P ->
   (H ==> H') ->
   H ==> (\[P] \* H').
-Proof. introv HP W. intros h K. rewrite* hstar_hpure_l. Qed.
+Proof using. introv HP W. intros h K. rewrite* hstar_hpure_l. Qed.
+
+Lemma hpure_inv_hempty : forall P h,
+  \[P] h ->
+  P /\ \[] h.
+Proof using.
+  introv M. rewrite <- hstar_hpure_l. rewrite~ hstar_hempty_r.
+Qed.
+
+Lemma hpure_intro_hempty : forall P h,
+  \[] h ->
+  P ->
+  \[P] h.
+Proof using.
+  introv M N. rewrite <- (hstar_hempty_l \[P]). rewrite~ hstar_hpure_r.
+Qed.
+
+Lemma himpl_hempty_hpure : forall P,
+  P ->
+  \[] ==> \[P].
+Proof using. introv HP. intros h Hh. applys* hpure_intro_hempty. Qed.
 
 Lemma himpl_hstar_hpure_l : forall P H H',
   (P -> H ==> H') ->
   (\[P] \* H) ==> H'.
-Proof. introv W Hh. rewrite hstar_hpure_l in Hh. applys* W. Qed.
+Proof using.
+  introv W Hh. rewrite hstar_hpure_l in Hh. applys* W.
+Qed.
 
-(* ================================================================= *)
-(** ** Properties of [hexists] *)
+Lemma hempty_eq_hpure_true :
+  \[] = \[True].
+Proof using.
+  applys himpl_antisym; intros h M.
+  { applys* hpure_intro_hempty. }
+  { forwards*: hpure_inv_hempty M. }
+Qed.
+
+Lemma hfalse_hstar_any : forall H,
+  \[False] \* H = \[False].
+Proof using.
+  intros. applys himpl_antisym; intros h; rewrite hstar_hpure_l; intros M.
+  { false*. } { lets: hpure_inv_hempty M. false*. }
+Qed.
+
+(* ----------------------------------------------------------------- *)
+(** *** Properties of [hexists] *)
+
+Lemma hexists_intro : forall A (x:A) (J:A->hprop) h,
+  J x h ->
+  (hexists J) h.
+Proof using. intros. exists~ x. Qed.
+
+Lemma hexists_inv : forall A (J:A->hprop) h,
+  (hexists J) h ->
+  exists x, J x h.
+Proof using. intros. destruct H as [x H]. exists~ x. Qed.
 
 Lemma himpl_hexists_l : forall A H (J:A->hprop),
   (forall x, J x ==> H) ->
   (hexists J) ==> H.
-Proof. introv W. intros h (x&Hh). applys* W. Qed.
+Proof using. introv W. intros h (x&Hh). applys* W. Qed.
 
 Lemma himpl_hexists_r : forall A (x:A) H J,
   (H ==> J x) ->
   H ==> (hexists J).
-Proof. introv W. intros h. exists x. apply* W. Qed.
+Proof using. introv W. intros h. exists x. apply~ W. Qed.
 
 Lemma himpl_hexists : forall A (J1 J2:A->hprop),
   J1 ===> J2 ->
   hexists J1 ==> hexists J2.
-Proof.
+Proof using.
   introv W. applys himpl_hexists_l. intros x. applys himpl_hexists_r W.
 Qed.
 
-(* ================================================================= *)
-(** ** Properties of [hforall] *)
+(* ----------------------------------------------------------------- *)
+(** *** Properties of [hforall] *)
+
+Lemma hforall_intro : forall A (J:A->hprop) h,
+  (forall x, J x h) ->
+  (hforall J) h.
+Proof using. introv M. applys* M. Qed.
+
+Lemma hforall_inv : forall A (J:A->hprop) h,
+  (hforall J) h ->
+  forall x, J x h.
+Proof using. introv M. applys* M. Qed.
 
 Lemma himpl_hforall_r : forall A (J:A->hprop) H,
   (forall x, H ==> J x) ->
   H ==> (hforall J).
-Proof. introv M. intros h Hh x. apply* M. Qed.
+Proof using. introv M. intros h Hh x. apply~ M. Qed.
 
 Lemma himpl_hforall_l : forall A x (J:A->hprop) H,
   (J x ==> H) ->
   (hforall J) ==> H.
-Proof. introv M. intros h Hh. apply* M. Qed.
+Proof using. introv M. intros h Hh. apply~ M. Qed.
+
+Lemma hforall_specialize : forall A (x:A) (J:A->hprop),
+  (hforall J) ==> (J x).
+Proof using. intros. applys* himpl_hforall_l x. Qed.
 
 Lemma himpl_hforall : forall A (J1 J2:A->hprop),
   J1 ===> J2 ->
   hforall J1 ==> hforall J2.
-Proof.
+Proof using.
   introv W. applys himpl_hforall_r. intros x. applys himpl_hforall_l W.
 Qed.
 
-(* ================================================================= *)
-(** ** Properties of [hsingle] *)
+(* ----------------------------------------------------------------- *)
+(** *** Properties of [hwand] *)
 
-Lemma hstar_hsingle_same_loc : forall p v1 v2,
-  (p ~~> v1) \* (p ~~> v2) ==> \[False].
-Proof.
+Lemma hwand_equiv : forall H0 H1 H2,
+  (H0 ==> H1 \-* H2) <-> (H1 \* H0 ==> H2).
+Proof using.
+  unfold hwand. iff M.
+  { rewrite hstar_comm. applys himpl_hstar_trans_l (rm M).
+    rewrite hstar_hexists. applys himpl_hexists_l. intros H.
+    rewrite (hstar_comm H). rewrite hstar_assoc.
+    rewrite (hstar_comm H H1). applys~ himpl_hstar_hpure_l. }
+  { applys himpl_hexists_r H0.
+    rewrite <- (hstar_hempty_r H0) at 1.
+    applys himpl_frame_r. applys himpl_hempty_hpure M. }
+Qed.
+
+Lemma himpl_hwand_r : forall H1 H2 H3,
+  H2 \* H1 ==> H3 ->
+  H1 ==> (H2 \-* H3).
+Proof using. introv M. rewrite~ hwand_equiv. Qed.
+
+Lemma himpl_hwand_r_inv : forall H1 H2 H3,
+  H1 ==> (H2 \-* H3) ->
+  H2 \* H1 ==> H3.
+Proof using. introv M. rewrite~ <- hwand_equiv. Qed.
+
+Lemma hwand_cancel : forall H1 H2,
+  H1 \* (H1 \-* H2) ==> H2.
+Proof using. intros. applys himpl_hwand_r_inv. applys himpl_refl. Qed.
+
+Arguments hwand_cancel : clear implicits.
+
+Lemma himpl_hempty_hwand_same : forall H,
+  \[] ==> (H \-* H).
+Proof using. intros. apply himpl_hwand_r. rewrite~ hstar_hempty_r. Qed.
+
+Lemma hwand_hempty_l : forall H,
+  (\[] \-* H) = H.
+Proof using.
+  intros. applys himpl_antisym.
+  { rewrite <- hstar_hempty_l at 1. applys hwand_cancel. }
+  { rewrite hwand_equiv. rewrite~ hstar_hempty_l. }
+Qed.
+
+Lemma hwand_hpure_l : forall P H,
+  P ->
+  (\[P] \-* H) = H.
+Proof using.
+  introv HP. applys himpl_antisym.
+  { lets K: hwand_cancel \[P] H. applys himpl_trans K.
+    applys* himpl_hstar_hpure_r. }
+  { rewrite hwand_equiv. applys* himpl_hstar_hpure_l. }
+Qed.
+
+Lemma hwand_curry : forall H1 H2 H3,
+  (H1 \* H2) \-* H3 ==> H1 \-* (H2 \-* H3).
+Proof using.
+  intros. apply himpl_hwand_r. apply himpl_hwand_r.
+  rewrite <- hstar_assoc. rewrite (hstar_comm H1 H2).
+  applys hwand_cancel.
+Qed.
+
+Lemma hwand_uncurry : forall H1 H2 H3,
+  H1 \-* (H2 \-* H3) ==> (H1 \* H2) \-* H3.
+Proof using.
+  intros. rewrite hwand_equiv. rewrite (hstar_comm H1 H2).
+  rewrite hstar_assoc. applys himpl_hstar_trans_r.
+  { applys hwand_cancel. } { applys hwand_cancel. }
+Qed.
+
+Lemma hwand_curry_eq : forall H1 H2 H3,
+  (H1 \* H2) \-* H3 = H1 \-* (H2 \-* H3).
+Proof using.
+  intros. applys himpl_antisym.
+  { applys hwand_curry. }
+  { applys hwand_uncurry. }
+Qed.
+
+Lemma hwand_inv : forall h1 h2 H1 H2,
+  (H1 \-* H2) h2 ->
+  H1 h1 ->
+  Fmap.disjoint h1 h2 ->
+  H2 (h1 \u h2).
+Proof using.
+  introv M2 M1 D. unfolds hwand. lets (H0&M3): hexists_inv M2.
+  lets (h0&h3&P1&P3&D'&U): hstar_inv M3. lets (P4&E3): hpure_inv P3.
+  subst h2 h3. rewrite union_empty_r in *. applys P4. applys* hstar_intro.
+Qed.
+
+(* ----------------------------------------------------------------- *)
+(** *** Properties of qwand *)
+
+Lemma qwand_equiv : forall H A (Q1 Q2:A->hprop),
+  H ==> (Q1 \--* Q2) <-> (Q1 \*+ H) ===> Q2.
+Proof using.
+  unfold qwand. iff M.
+  { intros x. rewrite hstar_comm. applys himpl_hstar_trans_l (rm M).
+    applys himpl_trans. applys hstar_hforall. simpl.
+    applys himpl_hforall_l x. rewrite hstar_comm. applys hwand_cancel. }
+  { applys himpl_hforall_r. intros x. rewrite* hwand_equiv. }
+Qed.
+
+Lemma qwand_cancel : forall A (Q1 Q2:A->hprop),
+  Q1 \*+ (Q1 \--* Q2) ===> Q2.
+Proof using. intros. rewrite <- qwand_equiv. applys qimpl_refl. Qed.
+
+Lemma himpl_qwand_r : forall A (Q1 Q2:A->hprop) H,
+  Q1 \*+ H ===> Q2 ->
+  H ==> (Q1 \--* Q2).
+Proof using. introv M. rewrite~ qwand_equiv. Qed.
+
+Arguments himpl_qwand_r [A].
+
+Lemma qwand_specialize : forall A (x:A) (Q1 Q2:A->hprop),
+  (Q1 \--* Q2) ==> (Q1 x \-* Q2 x).
+Proof using. intros. applys* himpl_hforall_l x. Qed.
+
+Arguments qwand_specialize [ A ].
+
+(* ----------------------------------------------------------------- *)
+(** *** Properties of [htop] *)
+
+Lemma htop_intro : forall h,
+  \Top h.
+Proof using. intros. exists~ (=h). Qed.
+
+Lemma himpl_htop_r : forall H,
+  H ==> \Top.
+Proof using. intros. intros h Hh. applys* htop_intro. Qed.
+
+Lemma htop_eq :
+  \Top = (\exists H, H).
+Proof using. auto. Qed.
+
+Lemma hstar_htop_htop :
+  \Top \* \Top = \Top.
+Proof using.
+  applys himpl_antisym.
+  { applys himpl_htop_r. }
+  { rewrite <- hstar_hempty_r at 1. applys himpl_frame_r. applys himpl_htop_r. }
+Qed.
+
+(* ----------------------------------------------------------------- *)
+(** *** Properties of [hsingle] *)
+
+Lemma hsingle_intro : forall p v,
+  (p ~~> v) (Fmap.single p v).
+Proof using. intros. hnfs*. Qed.
+
+Lemma hsingle_inv: forall p v h,
+  (p ~~> v) h ->
+  h = Fmap.single p v.
+Proof using. auto. Qed.
+
+Lemma hstar_hsingle_same_loc : forall p w1 w2,
+  (p ~~> w1) \* (p ~~> w2) ==> \[False].
+Proof using.
   intros. unfold hsingle. intros h (h1&h2&E1&E2&D&E). false.
   subst. applys* Fmap.disjoint_single_single_same_inv.
 Qed.
 
-(* ================================================================= *)
-(** ** Basic Tactics for Simplifying Entailments *)
+Arguments hstar_hsingle_same_loc : clear implicits.
 
-(** [xsimpl] performs immediate simplifications on entailment relations. *)
+(* ----------------------------------------------------------------- *)
+(** *** Definition and Properties of [haffine] and [hgc] *)
 
-#[global] Hint Rewrite hstar_assoc hstar_hempty_l hstar_hempty_r : hstar.
+Definition haffine (H:hprop) :=
+  True.
 
-Tactic Notation "xsimpl" :=
-  try solve [ apply qimpl_refl ];
-  try match goal with |- _ ===> _ => intros ? end;
-  autorewrite with hstar; repeat match goal with
-  | |- ?H \* _ ==> ?H \* _ => apply himpl_frame_r
-  | |- _ \* ?H ==> _ \* ?H => apply himpl_frame_l
-  | |- _ \* ?H ==> ?H \* _ => rewrite hstar_comm; apply himpl_frame_r
-  | |- ?H \* _ ==> _ \* ?H => rewrite hstar_comm; apply himpl_frame_l
-  | |- ?H ==> ?H => apply himpl_refl
-  | |- ?H ==> ?H' => is_evar H'; apply himpl_refl end.
+Lemma haffine_hany : forall (H:hprop),
+  haffine H.
+Proof using. unfold haffine. auto. Qed.
 
-Tactic Notation "xsimpl" "*" := xsimpl; auto_star.
+Lemma haffine_hempty :
+  haffine \[].
+Proof using. applys haffine_hany. Qed.
 
-(** [xchange] helps rewriting in entailments. *)
+Definition hgc := (* equivalent to [\exists H, \[haffine H] \* H] *)
+  htop.
 
-Lemma xchange_lemma : forall H1 H1',
-  H1 ==> H1' -> forall H H' H2,
-  H ==> H1 \* H2 ->
-  H1' \* H2 ==> H' ->
-  H ==> H'.
-Proof.
-  introv M1 M2 M3. applys himpl_trans M2. applys himpl_trans M3.
-  applys himpl_frame_l. applys M1.
-Qed.
+Notation "\GC" := (hgc) : hprop_scope.
 
-Tactic Notation "xchange" constr(M) :=
-  forwards_nounfold_then M ltac:(fun K =>
-    eapply xchange_lemma; [ eapply K | xsimpl | ]).
+Lemma haffine_hgc :
+  haffine \GC.
+Proof using. applys haffine_hany. Qed.
 
-(* end LibSepMinimal *)
+Lemma himpl_hgc_r : forall H,
+  haffine H ->
+  H ==> \GC.
+Proof using. introv M. applys himpl_htop_r. Qed.
+
+Lemma hstar_hgc_hgc :
+  \GC \* \GC = \GC.
+Proof using. applys hstar_htop_htop. Qed.
+
+(* ----------------------------------------------------------------- *)
+(** *** Functor Instantiation to Obtain [xsimpl] *)
+
+End SepSimplArgs.
+
+(** We are now ready to instantiate the functor that defines [xsimpl].
+    Demos of [xsimpl] are presented in chapter [Himpl.v]. *)
+
+Module Export HS := LibSepSimpl.XsimplSetup(SepSimplArgs).
+
+Export SepSimplArgs.
+
+(** From now on, all operators have opaque definitions. *)
+
+Global Opaque hempty hpure hstar hsingle hexists hforall
+              hwand qwand htop hgc haffine.
+
+(** At this point, the tactic [xsimpl] is defined. There remains to customize
+    the tactic so that it recognizes the predicate [p ~~> v] in a special way
+    when performing simplifications. *)
+
+(** The tactic [xsimpl_hook_hsingle p v] operates as part of [xsimpl].
+    The specification that follows makes sense only in the context of the
+    presentation of the invariants of [xsimpl] described in [LibSepSimpl.v].
+    This tactic is invoked on goals of the form [Xsimpl (Hla, Hlw, Hlt) HR],
+    where [Hla] is of the form [H1 \* .. \* Hn \* \[]]. The tactic
+    [xsimpl_hook_hsingle p v] searches among the [Hi] for a heap predicate
+    of the form [p ~~> v']. If it finds one, it moves this [Hi] to the front,
+    just before [H1]. Then, it cancels it out with the [p ~~> v] that occurs
+    in [HR]. Otherwise, the tactic fails. *)
+
+Ltac xsimpl_hook_hsingle p :=
+  xsimpl_pick_st ltac:(fun H' =>
+    match H' with (hsingle p ?v') =>
+      constr:(true) end);
+  apply xsimpl_lr_cancel_eq;
+  [ xsimpl_lr_cancel_eq_repr_post tt | ].
+
+(** The tactic [xsimpl_hook] handles cancellation of heap predicates of the
+    form [p ~~> v]. It forces their cancellation against heap predicates of
+    the form [p ~~> w], by asserting the equality [v = w]. Note: this tactic
+    is later refined to also handle records. *)
+
+Ltac xsimpl_hook H ::=
+  match H with
+  | hsingle ?p ?v => xsimpl_hook_hsingle p
+  end.
+
+(** One last hack is to improve the [math] tactic so that it is able
+    to handle the [val_int] coercion in goals and hypotheses of the
+    form [val_int ?n = val_int ?m], and so that it is able to process
+    the well-founded relations [dowto] and [upto] for induction on
+    integers. *)
+
+(* Ltac math_0 ::=
+  unfolds downto, upto;
+  repeat match goal with
+  | |- val_int _ = val_int _ => fequal
+  | H: val_int _ = val_int _ |- _ => inverts H
+  end. *)
+
+(* end LibSepReference *)
 
 Definition precond := hprop.
 Definition postcond := val -> hprop.
@@ -521,33 +874,33 @@ Definition env := ident -> option ufun.
 
 Inductive satisfies : env -> flow -> heap -> heap -> result -> Prop :=
 
-  | s_req : forall env p h1 h2 r,
-    (exists h3, h1 = Fmap.union h2 h3 /\ Fmap.disjoint h2 h3 /\ p h3) ->
+  | s_req env p h1 h2 r
+    (H: exists h3, h1 = Fmap.union h2 h3 /\ Fmap.disjoint h2 h3 /\ p h3) :
     satisfies env (req p) h1 h2 r
 
-  | s_ens : forall env q h1 h2 r,
-    (exists v h3, r = norm v /\ q v h3 /\ h2 = Fmap.union h1 h3 /\ Fmap.disjoint h1 h3) ->
+  | s_ens env q h1 h2 r
+    (H: exists v h3, r = norm v /\ q v h3 /\ h2 = Fmap.union h1 h3 /\ Fmap.disjoint h1 h3) :
     satisfies env (ens q) h1 h2 r
 
-  | s_seq : forall env f1 f2 h1 h2 r,
-    (exists h3 r1, satisfies env f1 h1 h3 r1 /\ satisfies env f2 h3 h2 r) -> satisfies env (seq f1 f2) h1 h2 r
+  | s_seq env f1 f2 h1 h2 r
+    (H: exists h3 r1, satisfies env f1 h1 h3 r1 /\ satisfies env f2 h3 h2 r) : satisfies env (seq f1 f2) h1 h2 r
 
   (* | s_ffex (a:Type) (f:a->flow) : forall env h1 h2 r x, *)
-  | s_ffex : forall env f h1 h2 r,
-    (exists v, satisfies env (f v) h1 h2 r) ->
+  | s_ffex env f h1 h2 r
+    (H: exists v, satisfies env (f v) h1 h2 r) :
     satisfies env (ffex f) h1 h2 r
 
-  | s_unk : forall env fn h1 h2 r f x,
-    env fn = Some f ->
-    satisfies env (f x r) h1 h2 (norm r) ->
+  | s_unk env fn h1 h2 r f x
+    (He: env fn = Some f)
+    (Hr: satisfies env (f x r) h1 h2 (norm r)) :
     satisfies env (unk fn x r) h1 h2 (norm r)
 
-  | s_disj_l : forall env h1 h2 r f1 f2,
-    satisfies env f1 h1 h2 r ->
+  | s_disj_l env h1 h2 r f1 f2
+    (H: satisfies env f1 h1 h2 r) :
     satisfies env (disj f1 f2) h1 h2 r
 
-  | s_disj_r : forall env h1 h2 r f1 f2,
-    satisfies env f2 h1 h2 r ->
+  | s_disj_r env h1 h2 r f1 f2
+    (H: satisfies env f2 h1 h2 r) :
     satisfies env (disj f1 f2) h1 h2 r
 
   .
@@ -590,65 +943,24 @@ Lemma req_sep_combine : forall H1 H2,
 Proof.
   unfold entails.
   intros.
-  inv H.
-  destruct H6 as (h3 & r1 & H1 & H2).
-  (* h3 is the heap after taking away the part satisfying P *)
-  
-  inv H1.
-  inv H2.
+  inverts H as H.
+  destruct H as (h3 & r1 & H3 & H4).
+
+  inverts H3 as H3.
+  inverts H4 as H4.
   destruct H3 as (h4 & ? & ? & ?).
-  destruct H1 as (h5 & ? & ? & ?).
+  destruct H4 as (h5 & ? & ? & ?).
   (* h4 is the part satisfying P, same for h5/Q *)
   constructor.
   (* union h4/h5 to get the part satisfying P*Q *)
-  (* TODO *)
-  assert (hdisjoint h4 h5).
-  (* Search hdisjoint. *)
-  (* Search hunion. *)
-  (* Search (hunion ?a _ = hunion ?a _). *)
-  subst h3.
-  rewrite hdisjoint_union_l in H0.
-  destruct H0.
-  rewrite hdisjoint_sym in H1.
-  easy.
 
-  exists (hunion h4 h5).
+  exists (h4 \+ h5).
+  subst h1 h3.
+  rew_disjoint.
+  (* fmap_disjoint. *)
   intuition.
-  subst h3.
-  rewrite hunion_assoc in H.
-  rewrite H.
-  (* rewrite <- hunion_invert_r. *)
-  assert (hunion h4 h5 = hunion h5 h4). rewrite hunion_comm. reflexivity.
-  apply hdisjoint_sym.
-  easy.
-  
-  rewrite H1.
-  reflexivity.
-
-  
-  rewrite hdisjoint_union_r.
-
-  intuition.
-
-  subst h3.
-  rewrite hdisjoint_union_l in H0.
-  intuition.
-
-  unfold sepconj.
-  exists h4. exists h5.
-
-  intuition.
-
-  (* unfold bientails. *)
-  (* split. *)
-  (* intros. *)
-  (* h1 is initial heap *)
-  (* h2 is final *)
-  (* h3 is the part taken off by P * Q *)
-  (* { inv H. destruct H2 as (h3 & H1 & H2 & H3).
-    constructor.
-    admit. } *)
-  (* { admit. } *)
+  fmap_eq.
+  apply hstar_intro; easy.
 Qed.
 
 (* Lemma req_sep : forall P Q,
@@ -673,7 +985,7 @@ Definition flow_res (f:flow) (v:val) : Prop :=
 (* Definition replace_ret (v:val) (f:flow) : flow :=
   f ;; ens (fun r => pure (r = v)). *)
 
-Definition empty := ens (fun r => pure True).
+Definition empty := ens (fun r => \[True]).
 
 Definition empty_env : env := fun _ => None.
 
@@ -740,7 +1052,7 @@ Qed. *)
 
 (* solve a heap goal.
   termination is guaranteed by ordering of lemmas to use *)
-Ltac hstep :=
+(* Ltac hstep :=
   match goal with
   (* | [ H: _ = hunion hempty _ |- _ ] =>
       rewrite hunion_empty in H
@@ -763,89 +1075,78 @@ Ltac hstep :=
       rewrite hunion_comm;
       rewrite hunion_empty *)
   (* | [ |- ?g ] => idtac *)
-  end.
+  end. *)
 
 
 Module SemanticsExamples.
 
-  Definition f1 : flow := ens (fun r => pure (r=vint 1)).
+  Definition f1 : flow := ens (fun r => \[r=vint 1]).
   Definition f2 : flow := fex (fun x => req (fun h => x = vint 1)).
   Definition f3 : flow := f1 ;; f2.
 
-  Example ex1: forall h, satisfies empty_env f1 h h (norm (vint 1)).
+  Example ex1: satisfies empty_env f1 Fmap.empty Fmap.empty (norm (vint 1)).
   Proof.
     intros.
     unfold f1.
-    (* fintro. *)
     apply s_ens.
     econstructor. eexists. intuition.
-    (* fintro. *)
-    unfold pure. intuition.
-    rewrite hunion_comm.
-    rewrite hunion_empty.
+    apply hpure_intro_hempty.
+    apply hempty_intro.
     reflexivity.
-    apply hdisjoint_empty.
-    rewrite hdisjoint_sym.
-    apply hdisjoint_empty.
-    (* hstep. *)
-    (* hstep. *)
+    fmap_eq.
   Qed.
 
   Example ex2_ret: flow_res f1 (vint 1).
   Proof.
     unfold flow_res.
-    exists hempty. exists hempty.
+
+    exists empty_heap.
+    exists empty_heap.
     exists empty_env.
     unfold f1.
-    (* fintro. *)
     econstructor. eexists. eexists. intuition.
-    (* fintro. *)
-    unfold pure. intuition.
-    hstep.
-    hstep.
+    apply hpure_intro_hempty.
+    apply hempty_intro.
+    reflexivity.
+    fmap_eq.
   Qed.
 
   Example ex3_req_ret: flow_res f2 (vint 2).
   Proof.
     unfold flow_res.
-    exists hempty.
-    exists hempty.
+    exists empty_heap.
+    exists empty_heap.
     exists empty_env.
     unfold f2.
-    (* eexists. *)
-    (* fexists (vint 1). *)
-    (* unfold req. *)
     apply (s_ffex).
     eexists.
     constructor.
     eexists.
-    (* exists hempty. *)
     intuition.
-    rewrite hunion_empty.
-    auto.
-    apply hdisjoint_empty.
-    (* hstep. *)
-    (* hstep. *)
+    fmap_eq.
   Qed.
 
   Definition f4 : flow := empty ;; fex (fun r => unk "f" (vint 1) r).
-  Definition f4_env : env := eupdate "f" (fun _ r => ens (fun r1 => pure (r = vint 2))) empty_env.
+  Definition f4_env : env := eupdate "f" (fun _ r => ens (fun r1 => \[r = vint 2])) empty_env.
 
   (* has to be 2 *)
   Example ex5_f_ret: flow_res f4 (vint 2).
   Proof.
     unfold flow_res.
-    exists hempty. exists hempty. exists f4_env.
+    exists empty_heap. exists empty_heap. exists f4_env.
     unfold f4.
     (* fintro. *)
-    constructor. exists hempty. exists (norm (vint 7)). intuition.
+    constructor. exists empty_heap. exists (norm (vint 7)). intuition.
     (* fintro. *)
     constructor.
     eexists.
-    exists hempty.
-    unfold pure. intuition.
-    hstep.
-    hstep.
+    exists empty_heap.
+    intuition.
+    apply hpure_intro_hempty.
+    apply hempty_intro.
+    easy.
+    fmap_eq.
+
     constructor.
     exists (vint 2).
     econstructor.
@@ -853,15 +1154,16 @@ Module SemanticsExamples.
     apply eupdate_same.
     constructor.
     exists (vint 2).
-    exists hempty.
+    exists empty_heap.
     intuition.
-    unfold pure.
-    intuition.
-    hstep.
-    hstep.
+
+    apply hpure_intro_hempty.
+    apply hempty_intro.
+    reflexivity.
+    fmap_eq.
   Qed.
 
-  Example ex4: forall h, satisfies (eupdate "f" (fun x r1 => ens (fun r => pure (r1 = r /\ r = x))) empty_env) f4 h h (norm (vint 1)).
+  Example ex4: forall h, satisfies (eupdate "f" (fun x r1 => ens (fun r => \[r1 = r /\ r = x])) empty_env) f4 h h (norm (vint 1)).
   Proof.
     intros.
     constructor.
@@ -870,11 +1172,13 @@ Module SemanticsExamples.
     split.
     - constructor.
     eexists.
-    exists hempty.
+    exists empty_heap.
     intuition.
-    unfold pure. intuition.
-    hstep.
-    hstep.
+
+    apply hpure_intro_hempty.
+    apply hempty_intro.
+    easy.
+    fmap_eq.
     -
     eapply s_ffex.
     exists (vint 1).
@@ -887,16 +1191,16 @@ Module SemanticsExamples.
 
     constructor.
     eexists.
-    exists hempty.
+    exists empty_heap.
     intuition.
-    unfold pure.
+    apply hpure_intro_hempty.
+    apply hempty_intro.
     intuition.
-    hstep.
-    hstep.
+    fmap_eq.
   Qed.
 
-  Definition f5 : flow := ens (fun r => pure (r = vint 2)).
-  Definition f6 : flow := f1 ;; ens (fun r => pure (r = vint 2)).
+  Definition f5 : flow := ens (fun r => \[r = vint 2]).
+  Definition f6 : flow := f1 ;; ens (fun r => \[r = vint 2]).
 
   Example ex6_ent : f5 ⊑ f6.
   Proof.
@@ -915,27 +1219,24 @@ Module SemanticsExamples.
     - unfold f1.
       constructor.
       exists (vint 1).
-      exists hempty.
+      exists empty_heap.
       intuition.
-      unfold pure.
+      apply hpure_intro_hempty.
+      apply hempty_intro.
       intuition.
-      hstep.
-      hstep.
-
+      fmap_eq.
     -
       constructor.
       eexists.
-      exists hempty.
+      exists empty_heap.
       intuition.
-      unfold pure.
+      apply hpure_intro_hempty.
+      apply hempty_intro.
+      apply hpure_inv in H2.
       intuition.
-      unfold pure in H2.
-      intuition auto.
-      unfold pure in H2.
-      destruct H2.
-      subst.
-      auto.
-      hstep.
+      apply hpure_inv in H2.
+      intuition.
+      fmap_eq.
   Qed.
  
   Example ex7_rewrite : f5 ⊑ f6.
@@ -945,7 +1246,7 @@ Module SemanticsExamples.
   Qed.
 
   Definition foldr :=
-  ens (fun _ => pure True) ;;
+  ens (fun _ => \[True]) ;;
   disj
     (unk "f" (vint 2) (vint 3))
     (unk "foldr" (vint 1) (vint 1);;
@@ -960,7 +1261,7 @@ End SemanticsExamples.
 (* forward rules say how to produce a staged formula from a program *)
 Inductive forward : expr -> flow -> Prop :=
   | fw_val: forall n,
-    forward (pval n) (ens (fun res => pure (res = n)))
+    forward (pval n) (ens (fun res => \[res = n]))
 
   (* there is no need for fw_var/a store because substitution will take care of it before it is reached *)
 
@@ -989,8 +1290,8 @@ Section ForwardExamples.
   (* let x = 1 in x *)
   Definition e1 := (plet "x" (pval (vint 1)) (pvar "x")).
   Definition f1 :=
-    ens (fun v => pure (v = vint 1)) ;;
-    ens (fun r => pure (r = vint 1)).
+    ens (fun v => \[v = vint 1]) ;;
+    ens (fun r => \[r = vint 1]).
 
   Example ex1:
     forward e1 f1.
@@ -998,8 +1299,8 @@ Section ForwardExamples.
     eapply fw_let.
     - apply fw_val.
     - unfold flow_res.
-      exists hempty.
-      exists hempty.
+      exists empty_heap.
+      exists empty_heap.
       exists empty_env.
       constructor.
       intuition.
@@ -1007,14 +1308,11 @@ Section ForwardExamples.
       eexists.
       eexists.
       auto.
-      unfold pure. intuition.
-      rewrite hunion_empty.
+      intuition.
+      apply hpure_intro_hempty.
+      apply hempty_intro.
       reflexivity.
-      apply hdisjoint_empty.
-      (* fintro.
-      fintro.
-      hstep.
-      hstep. *)
+      fmap_eq.
     - simpl.
       apply fw_val.
   Qed.
